Update mulitple files for exp_id related defs and thms

pancake/crepLangScript.sml
@@ -18,8 +18,6 @@ Type varname = ``:num``
 
 Type funname = ``:mlstring``
 
-(* Type eid = ``:num`` *)
-
 Datatype:
   exp = Const ('a word)
       | Var varname
@@ -206,46 +204,6 @@ Definition acc_vars_def:
       acc_vars rp (acc_vars ep nl)) ∧
   (acc_vars _ l = l)
 End
-
-(* specifying them as set for the time being *)
-Definition exp_ids_def:
-  (exp_ids Skip = ({}:'a word set)) ∧
-  (exp_ids (Raise eid) = {eid}) ∧
-  (exp_ids (Dec _ _ p) = exp_ids p) ∧
-  (exp_ids (Seq p q) = exp_ids p ∪ exp_ids q) ∧
-  (exp_ids (If _ p q) = exp_ids p ∪ exp_ids q) ∧
-  (exp_ids (While _ p) = exp_ids p) ∧
-  (exp_ids (Call (Ret _ rp NONE) _ _) = exp_ids rp) ∧
-  (exp_ids (Call (Ret _ rp (SOME (Handle w ep))) _ _) = {w} ∪ exp_ids rp ∪ exp_ids ep) ∧
-  (exp_ids _ = {})
-End
-
-(*
-Definition acc_vars_def:
-  (acc_vars Skip = ({}:num set)) ∧
-  (acc_vars (Dec n e p) = {n} ∪ set (var_cexp e) ∪ acc_vars p) ∧
-  (acc_vars (Assign n e) = {n} ∪ set (var_cexp e)) ∧
-  (acc_vars (Store e1 e2) = set (var_cexp e1) ∪ set (var_cexp e2)) ∧
-  (acc_vars (StoreByte e1 e2) = set (var_cexp e1) ∪ set (var_cexp e2)) ∧
-  (acc_vars (StoreGlob _ e) = set (var_cexp e)) ∧
-  (acc_vars (Seq p q) = acc_vars p ∪ acc_vars q) ∧
-  (acc_vars (If e p q) = set (var_cexp e) ∪ acc_vars p ∪ acc_vars q) ∧
-  (acc_vars (While e p) = set (var_cexp e) ∪ acc_vars p) ∧
-  (acc_vars (Return e) = set (var_cexp e)) ∧
-  (acc_vars (ExtCall f v1 v2 v3 v4) = {v1; v2; v3; v4}) ∧
-  (acc_vars (Call Tail trgt args) = set (var_cexp trgt) ∪ ARB (set (MAP var_cexp args))) ∧
-  (acc_vars (Call (Ret NONE rp NONE) trgt args) =
-       acc_vars rp ∪ set (var_cexp trgt) ∪ ARB (set (MAP var_cexp args))) ∧
-  (acc_vars (Call (Ret NONE rp (SOME (Handle w ep))) trgt args) =
-       acc_vars rp ∪  acc_vars ep ∪ set (var_cexp trgt) ∪ ARB (set (MAP var_cexp args))) ∧
-  (acc_vars (Call (Ret (SOME rv) rp NONE) trgt args) =
-       {rv} ∪ set (var_cexp trgt) ∪ ARB (set(MAP var_cexp args))) ∧
-  (acc_vars (Call (Ret (SOME rv) rp (SOME (Handle w ep))) trgt args) =
-        {rv} ∪ acc_vars rp ∪  acc_vars ep ∪ set (var_cexp trgt) ∪ ARB (set (MAP var_cexp args))) ∧
-  (acc_vars _ = {})
-End
-
-*)
 
 Overload shift = “backend_common$word_shift”
 
